H10/HALT_MM.v
@@ -17,12 +17,17 @@ From Undecidability.PCP Require Import singleTM TM_SRH SRH_SR SR_MPCP MPCP_PCP.
 
 Set Implicit Arguments.
 
-Corollary MM_HALTING_undec : Halt ⪯ MM_HALTING.
+Corollary Halt_PCP : Halt ⪯ PCP.
 Proof.
   eapply reduces_transitive. exact TM_SRH.Halt_SRH.
   eapply reduces_transitive. exact SRH_SR.reduction.
   eapply reduces_transitive. exact SR_MPCP.reduction.
-  eapply reduces_transitive. exact MPCP_PCP.reduction.
+  exact MPCP_PCP.reduction.
+Qed.
+
+Corollary MM_HALTING_undec : Halt ⪯ MM_HALTING.
+Proof.
+  eapply reduces_transitive. exact Halt_PCP.
   exact PCP_MM_HALTING.
 Qed.
 
